started on listSet abstraction for finite sets.  also on the burner is a finite-approximation well-founded galois connection (galois up to finite approximation)

src/FP/Data/List.v
@@ -6,45 +6,50 @@ Require Import FP.Classes.Traversable.
 Section Vanilla.
   Infix "v∷" := cons (at level 60, right associativity).
   Notation "v[ x , .. , y ]" := (cons x .. (cons y nil) ..).
-
-  Definition lmap {A B} (f:A -> B) : list A -> list B :=
+  
+  Definition vlmap {A B} (f:A -> B) : list A -> list B :=
     fix lmap xs :=
       match xs with
       | nil => nil
       | x v∷ xs => f x v∷ lmap xs
       end.
 
-  Inductive list_eqv {A} `{! Eqv A } : relation (list A) :=
-    | NullListEqv : list_eqv nil nil
-    | ConsListEqv : forall x y xs ys, x ≃ y -> list_eqv xs ys -> list_eqv (x v∷ xs) (y v∷ ys).
-  Inductive list_lte {A} `{! Eqv A ,! Lte A } : relation (list A) :=
-    | NullListLte : forall xs, list_lte nil xs
-    | ConsListLte : forall x y xs ys, x ⊑ y -> list_lte xs ys -> list_lte (x v∷ xs) (y v∷ ys).
-  Global Instance : forall A `{! Eqv A }, Eqv (list A) := { eqv := list_eqv }.
+  Inductive vlist_eqv {A} `{! Eqv A } : relation (list A) :=
+    | NullListEqv : vlist_eqv nil nil
+    | ConsListEqv : forall x y xs ys, x ≃ y -> vlist_eqv xs ys -> vlist_eqv (x v∷ xs) (y v∷ ys).
+  Inductive vlist_lte {A} `{! Eqv A ,! Lte A } : relation (list A) :=
+    | NullListLte : forall xs, vlist_lte nil xs
+    | ConsListLte : forall x y xs ys, x ⊑ y -> vlist_lte xs ys -> vlist_lte (x v∷ xs) (y v∷ ys).
+  Global Instance : forall A `{! Eqv A }, Eqv (list A) := { eqv := vlist_eqv }.
   Admitted.
-  Global Instance : forall A `{! Eqv A ,! Lte A }, Lte (list A) := { lte := list_lte }.
+  Global Instance : forall A `{! Eqv A ,! Lte A }, Lte (list A) := { lte := vlist_lte }.
   Admitted.
 End Vanilla.
 
-Definition qlist (A:qtype) : qtype := {| qdom := list (dom A) |}.
-Definition qnil {A} : dom (qlist A).
-Admitted.
-Definition qcons {A} : dom (A ⇒ qlist A ⇒ qlist A).
-Admitted.
-Definition qlist_elim {A B} : dom (qlist A ⇒ B ⇒ (A ⇒ B ⇒ B) ⇒ B).
-Admitted.
-Definition qinsert {A B} : dom (A ⇒ B ⇒ qlist (A × B) ⇒ qlist (A × B)).
-Admitted.
-Definition qlookup {A B} `{! DecEqv (dom A) } : dom (A ⇒ qlist (A × B) ⇒ qoption B).
-Admitted.
-Definition qzip {A B} : dom (qlist A ⇒ qlist B ⇒ qlist (A × B)).
-Admitted.
-Definition qunzip {A B} : dom (qlist (A × B) ⇒ qlist A × qlist B).
-Admitted.
-Definition qlmap {A B} : dom ((A ⇒ B) ⇒ qlist A ⇒ qlist B) := 
-  λ (f:dom (A ⇒ B)) (x:dom (qlist A)) → lmap (rfun f) x : dom (qlist B).
+Definition vlist := Coq.Init.Datatypes.list.
+Definition vnil {A} : vlist A := Coq.Init.Datatypes.nil.
+Definition vcons := Coq.Init.Datatypes.cons.
 
-Notation "x ∷ xs" := (qcons ∙ x ∙ xs) (at level 60, right associativity).
 
-Instance : Traversable qlist.
+Definition list (A:qtype) : qtype := {| qdom := vlist (dom A) |}.
+Definition nil {A} : dom (list A).
+Admitted.
+Definition cons {A} : dom (A ⇒ list A ⇒ list A).
+Admitted.
+Definition list_elim {A B} : dom (list A ⇒ B ⇒ (A ⇒ B ⇒ B) ⇒ B).
+Admitted.
+Definition linsert {A B} : dom (A ⇒ B ⇒ list (A × B) ⇒ list (A × B)).
+Admitted.
+Definition llookup {A B} `{! DecEqv (dom A) } : dom (A ⇒ list (A × B) ⇒ qoption B).
+Admitted.
+Definition zip {A B} : dom (list A ⇒ list B ⇒ list (A × B)).
+Admitted.
+Definition unzip {A B} : dom (list (A × B) ⇒ list A × list B).
+Admitted.
+Definition lmap {A B} : dom ((A ⇒ B) ⇒ list A ⇒ list B) := 
+  λ (f:dom (A ⇒ B)) (x:dom (list A)) → vlmap (rfun f) x : dom (list B).
+
+Notation "x ∷ xs" := (cons ∙ x ∙ xs) (at level 60, right associativity).
+
+Instance : Traversable list.
 Admitted.
